coq/thielemachine/coqproofs/Subsumption.v
@@ -1,6 +1,10 @@
-Require Import ThieleMachine.
+Require Import ThieleMachine.ThieleMachine.
 Require Import List String.
 Import ListNotations.
+
+Definition TMConfig := State.
+Definition TM := Prog.
+Definition tm_step := tm_step_fun.
 
 Module ThieleSubsumesTuring.
 
@@ -10,19 +14,35 @@ Record ThieleConfig := {
   mu_cost : nat;
 }.
 
-Definition thiele_step (tm : TM nat nat) (th_conf : ThieleConfig) : ThieleConfig :=
-  {| tm_config := tm_step tm th_conf.(tm_config);
-     ledger := "Step taken."%string :: th_conf.(ledger);
-     mu_cost := S th_conf.(mu_cost) |}.
+Definition thiele_step (tm : TM) (th_conf : ThieleConfig) : option ThieleConfig :=
+  match tm_step tm th_conf.(tm_config) with
+  | Some (next_state, _obs) =>
+      Some {|
+        tm_config := next_state;
+        ledger := "Step taken."%string :: th_conf.(ledger);
+        mu_cost := S th_conf.(mu_cost)
+      |}
+  | None => None
+  end.
 
 End ThieleSubsumesTuring.
 
 Theorem thiele_machine_subsumes_turing_machine :
-  forall (tm : TM nat nat) (conf : TMConfig),
-    (ThieleSubsumesTuring.thiele_step tm {| ThieleSubsumesTuring.tm_config := conf;
-                                            ThieleSubsumesTuring.ledger := [];
-                                            ThieleSubsumesTuring.mu_cost := 0 |}).(ThieleSubsumesTuring.tm_config)
-    = tm_step tm conf.
+  forall (tm : TM) (conf : TMConfig),
+    ThieleSubsumesTuring.thiele_step tm
+      {| ThieleSubsumesTuring.tm_config := conf;
+         ThieleSubsumesTuring.ledger := [];
+         ThieleSubsumesTuring.mu_cost := 0 |}
+    =
+    match tm_step tm conf with
+    | Some (next_state, _obs) =>
+        Some {|
+          ThieleSubsumesTuring.tm_config := next_state;
+          ThieleSubsumesTuring.ledger := ["Step taken."%string];
+          ThieleSubsumesTuring.mu_cost := 1
+        |}
+    | None => None
+    end.
 Proof.
   intros. reflexivity.
 Qed.
