coq/thielemachine/coqproofs/ListModules.v
@@ -1,0 +1,2 @@
+(* Minimal file to test logical path visibility *)
+Print Modules.
